theory/JIT_def.thy
@@ -1,0 +1,33 @@
+theory JIT_def
+imports
+  Main
+  rBPFCommType rBPFSyntax
+  x64Syntax
+  StepSem
+begin
+
+
+
+axiomatization x64_encode :: "instruction \<Rightarrow> x64_bin option"
+
+record CallFrame = (*  /// The caller saved registers
+    pub caller_saved_registers: [u64; ebpf::SCRATCH_REGS],
+*)
+caller_saved_registers :: "u64 list"
+frame_pointer :: u64
+target_pc :: u64
+
+record stack_state = 
+call_depth :: u64
+stack_pointer :: u64
+call_frames :: "CallFrame list"
+
+type_synonym func_key = u32
+
+type_synonym func_val = u64
+type_synonym func_map = "(func_key, func_val) map"
+
+
+
+
+end
