theory/StepSem.thy
@@ -5,4 +5,17 @@ begin
 inductive star::"('a \<Rightarrow> 'a \<Rightarrow> bool) \<Rightarrow> 'a \<Rightarrow> 'a \<Rightarrow> bool" for r where
 refl:"star r x x"|
 step: "r x y \<Longrightarrow> star r y z \<Longrightarrow> star r x z"
+
+
+lemma star_left:
+  "r s1 s2 \<Longrightarrow> star r s2 s3 \<Longrightarrow> star r s1 s3"
+  apply (rule star.step; simp)
+  done
+
+(*
+lemma star_right:
+  "star r s1 s2 \<Longrightarrow> r s2 s3 \<Longrightarrow> star r s1 s3"
+  apply (rule star.step [of _ _ s2])
+  done *)
+
 end
