theory/rBPFSem.thy
@@ -1,0 +1,58 @@
+theory rBPFSem
+imports
+    Main
+    rBPFCommType rBPFSyntax Mem
+begin
+
+type_synonym reg_map = "bpf_ireg \<Rightarrow> u64"
+
+
+definition eval_reg :: "dst_ty \<Rightarrow> reg_map \<Rightarrow> u64" where
+"eval_reg dst rs = rs dst"
+syntax "_upd_reg" :: "'a \<Rightarrow> 'b \<Rightarrow> 'c \<Rightarrow> 'a" ("_ # _ <-- _" [1000, 1000, 1000] 1)
+
+(* Define the translation for the notation *)
+translations
+  "_upd_reg a b c" => "a(b := c)"
+
+datatype sbpf_state =
+  SBPF_OK u64 reg_map mem (* stack_state SBPFV func_map u64 u64 *) | (**r normal state *)
+  SBPF_Success u64 |
+  SBPF_Err
+
+fun eval_snd_op_u64 :: "snd_op \<Rightarrow> reg_map \<Rightarrow> u64" where
+"eval_snd_op_u64 (SOImm i) _ = scast i" |
+"eval_snd_op_u64 (SOReg r) rs = rs r"
+
+definition eval_alu :: "binop \<Rightarrow> dst_ty \<Rightarrow> snd_op \<Rightarrow> reg_map \<Rightarrow> reg_map option" where
+"eval_alu bop dst sop rs = (
+  let dv :: u64 = eval_reg dst rs in (
+  let sv :: u64 = eval_snd_op_u64 sop rs in (
+  case bop of
+  BPF_ADD   \<Rightarrow> Some (rs#dst <-- (dv+sv)) |
+  _ \<Rightarrow> None
+)))"
+
+fun sbpf_step :: "ebpf_asm \<Rightarrow> sbpf_state \<Rightarrow> sbpf_state" where
+"sbpf_step prog (SBPF_OK pc rs m) = (
+  if length prog = 0 then SBPF_Err
+  else (
+    case prog!(unat pc) of
+    BPF_ALU64 bop d sop \<Rightarrow> (
+      case bop of
+      BPF_ADD \<Rightarrow>(
+        case eval_alu bop d sop rs of
+        None \<Rightarrow> SBPF_Err |
+        Some rs' \<Rightarrow> SBPF_OK (pc+1) rs' m
+      ) |
+    _ \<Rightarrow> SBPF_Err) |
+    BPF_EXIT \<Rightarrow> SBPF_Success (rs BR0) |
+    _ \<Rightarrow> SBPF_Err
+))" |
+"sbpf_step _ _ = SBPF_Err"
+
+fun sbpf_sem :: "nat \<Rightarrow> ebpf_asm \<Rightarrow> sbpf_state \<Rightarrow> sbpf_state" where
+"sbpf_sem 0 _ st = st" |
+"sbpf_sem (Suc n) prog st = sbpf_sem n prog (sbpf_step prog st)"
+
+end
