theory/x64Syntax.thy
@@ -1,0 +1,198 @@
+section \<open> x64 Syntax \<close>
+
+theory x64Syntax
+imports
+  Main
+  rBPFCommType Mem
+begin
+  
+subsection  \<open> x64 Syntax \<close>
+
+datatype ireg = RAX | RBX | RCX | RDX | RSI | RDI | RBP | RSP | R8 | R9 | R10 | R11 | R12 | R13 | R14 | R15
+
+(*
+fun u8_of_ireg ::"ireg \<Rightarrow> u8" where
+"u8_of_ireg RAX = 0" |
+"u8_of_ireg RBX = 1" |
+"u8_of_ireg RCX = 2" |
+"u8_of_ireg RDX = 3" |
+"u8_of_ireg RSI = 4" |
+"u8_of_ireg RDI = 5" |
+"u8_of_ireg RBP = 6" |
+"u8_of_ireg RSP = 7" |
+"u8_of_ireg R8  = 8" |
+"u8_of_ireg R9  = 9" |
+"u8_of_ireg R10 = 10" |
+"u8_of_ireg R11 = 11" |
+"u8_of_ireg R12 = 12" |
+"u8_of_ireg R13 = 13" |
+"u8_of_ireg R14 = 14" |
+"u8_of_ireg R15 = 15" *)
+
+text \<open> TODO: Solana rBPF uses the following mapping, very weird.
+I don't understand, see: https://github.com/solana-labs/rbpf/blob/main/src/x86.rs#L16 
+But this mapping doesn't effect x64 semantics, only binary code
+\<close>
+
+fun u8_of_ireg ::"ireg \<Rightarrow> u8" where
+"u8_of_ireg RAX = 0" |
+"u8_of_ireg RCX = 1" |
+"u8_of_ireg RDX = 2" |
+"u8_of_ireg RBX = 3" |
+"u8_of_ireg RSP = 4" | 
+"u8_of_ireg RBP = 5" |
+"u8_of_ireg RSI = 6" |
+"u8_of_ireg RDI = 7" |
+"u8_of_ireg R8  = 8" |        
+"u8_of_ireg R9  = 9" |
+"u8_of_ireg R10 = 10" |
+"u8_of_ireg R11 = 11" |
+"u8_of_ireg R12 = 12" |
+"u8_of_ireg R13 = 13" |
+"u8_of_ireg R14 = 14" |
+"u8_of_ireg R15 = 15"
+
+definition ireg_of_u8 ::"u8 \<Rightarrow> ireg option" where
+"ireg_of_u8 i = (                
+        if i = 0 then
+    Some RAX
+  else  if i = 1 then
+    Some RCX
+  else  if i = 2 then
+    Some RDX
+  else  if i = 3 then
+    Some RBX
+  else  if i = 4 then
+    Some RSP
+  else  if i = 5 then
+    Some RBP
+  else  if i = 6 then
+    Some RSI
+  else  if i = 7 then
+    Some RDI
+  else  if i = 8 then
+    Some R8
+  else  if i = 9 then
+    Some R9
+  else  if i = 10 then
+    Some R10
+  else  if i = 11 then
+    Some R11
+  else  if i = 12 then
+    Some R12
+  else  if i = 13 then
+    Some R13
+  else  if i = 14 then
+    Some R14
+  else  if i = 15 then
+    Some R15
+  else
+    None
+)"
+
+text \<open> skip float registers, as Solana rBPF doesn't deal with float \<close>
+
+datatype crbit = ZF | CF | PF | SF | OF
+
+(*
+datatype preg = PC | IR ireg | CR crbit
+
+abbreviation "RIP \<equiv> PC"  \<comment> \<open> the RIP register in x86-64 (x64) architecture is the equivalent of the program counter (PC) in many other architectures.  \<close>
+    *)
+
+abbreviation "SP \<equiv> RSP"
+
+type_synonym label = nat
+
+datatype addrmode =
+  Addrmode "ireg option" "(ireg * u8) option" u32
+
+datatype testcond =
+    Cond_e | Cond_ne
+  | Cond_b | Cond_be | Cond_ae | Cond_a
+  | Cond_l | Cond_le | Cond_ge | Cond_g
+  | Cond_p | Cond_np
+
+fun u8_of_cond :: "testcond \<Rightarrow> u8" where
+"u8_of_cond Cond_b  = 2" |  (* B, NAE: Below, Not above or equal *)
+"u8_of_cond Cond_ae = 3" |  (* NB, AE: Not below, Above or equal *)
+"u8_of_cond Cond_e  = 4" |  (* E, Z: Equal, Zero *)
+"u8_of_cond Cond_ne = 5" |  (* NE, NZ: Not equal, Not zero *)
+"u8_of_cond Cond_be = 6" |  (* BE, NA: Below or equal, Not above *)
+"u8_of_cond Cond_a  = 7" |  (* NBE, A: Not below or equal, Above *)
+"u8_of_cond Cond_p  = 10" | (* P, PE: Parity, Parity Even *)
+"u8_of_cond Cond_np = 11" | (* NP, PO: Not parity, Parity Odd *)
+"u8_of_cond Cond_l  = 12" | (* L, NGE: Less than, Not greater than or equal *)
+"u8_of_cond Cond_ge = 13" | (* NL, GE: Not less than, Greater than or equal to *)
+"u8_of_cond Cond_le = 14" | (* LE, NG: Less than or equal to, Not greater than *)
+"u8_of_cond Cond_g  = 15"   (* NLE, G: Not less than or equal to, Greater*)
+
+definition cond_of_u8 :: "u8 \<Rightarrow> testcond option" where
+"cond_of_u8 i = (
+  if i = 2 then
+    Some Cond_b
+  else  if i = 3 then
+    Some Cond_ae
+  else  if i = 4 then
+    Some Cond_e
+  else  if i = 5 then
+    Some Cond_ne
+  else  if i = 6 then
+    Some Cond_be
+  else  if i = 7 then
+    Some Cond_a
+  else  if i = 10 then
+    Some Cond_p
+  else  if i = 11 then
+    Some Cond_np
+  else  if i = 12 then
+    Some Cond_l
+  else  if i = 13 then
+    Some Cond_ge
+  else  if i = 14 then
+    Some Cond_le
+  else  if i = 15 then
+    Some Cond_g
+  else
+    None
+)"
+
+(** Instructions.  IA32 instructions accept many combinations of
+  registers, memory references and immediate constants as arguments.
+  Here, we list only the combinations that we actually use.
+
+  Naming conventions for types: Pmov_rm   rd a c  \<Rightarrow> exec_store  sz c m a rs (IR rd) [] |                 \<comment> \<open> load  mem to reg \<close>
+  Pmov_mr   a r1 c  \<Rightarrow> exec_load   sz c m a rs (IR r1) |            
+- [b]: 8 bits
+- [w]: 16 bits ("word")
+- [l]: 32 bits ("longword")
+- [q]: 64 bits ("quadword")
+- [d] or [sd]: FP double precision (64 bits)
+- [s] or [ss]: FP single precision (32 bits)
+
+  Naming conventions for operands:
+- [r]: integer register operand
+- [f]: XMM register operand
+- [m]: memory operand
+- [i]: immediate integer operand
+- [s]: immediate symbol operand
+- [l]: immediate label operand
+- [cl]: the [CL] register
+
+  For two-operand instructions, the first suffix describes the result
+  (and first argument), the second suffix describes the second argument.
+*)
+
+datatype instruction =
+  Paddq_rr ireg ireg
+  | Pret
+  | Pnop
+
+
+type_synonym x64_asm = "instruction list"
+type_synonym x64_bin = "u8 list"
+
+lemma u8_of_ireg_of_u8_iff: "(u8_of_ireg r = i) = (ireg_of_u8 i = Some r)"
+  by (cases r, auto simp add: ireg_of_u8_def)
+
+end
