ROOT
@@ -1,4 +1,4 @@
 session Solana_rBPF = Main +
   options [timeout = 600]
   theories
-    JIT_abs
+    JIT
